Lean4Lean/Verify/EquivManager.lean
@@ -326,7 +326,7 @@ theorem addEquiv.WF {c : VContext} {s : VState} (he₁ : c.TrExprS e₁ e') (he�
 
 theorem isDefEq.WF {c : VContext} {s : VState}
     (he₁ : c.TrExprS e₁ e₁') (he₂ : c.TrExprS e₂ e₂') :
-    RecM.WF c s (isDefEq e₁ e₂) fun b _ => b → c.IsDefEqU e₁' e₂' := by
+    RecM.WF c s (isDefEq e₁ e₂ tag) fun b _ => b → c.IsDefEqU e₁' e₂' := by
   refine (isDefEqCore.WF he₁ he₂).bind fun b _ _ hb => ?_
   simp; split
   · exact (addEquiv.WF he₁ ⟨_, he₂, (hb ‹_›).symm⟩).map fun _ _ _ _ => hb
